"state" end2end theorem

compiler/src/examples/FE310Compiler.v
@@ -4,7 +4,12 @@ Require Import coqutil.Decidable.
 Require Import compiler.ExprImp.
 Require Import compiler.NameGen.
 Require Import compiler.Pipeline.
-Require Import compiler.Basic32Semantics.
+Require Import Coq.ZArith.ZArith.
+Require Import coqutil.Map.SortedList.
+Require Import riscv.Words32Naive.
+Require Import riscv.DefaultMemImpl32.
+Require Import coqutil.Map.Empty_set_keyed_map.
+Require Import coqutil.Map.Z_keyed_SortedListMap.
 Require Import riscv.util.Monads.
 Require Import compiler.util.Common.
 Require        riscv.InstructionNotations.
@@ -25,6 +30,8 @@ Open Scope Z_scope.
 Notation RiscvMachine := (RiscvMachine Register MMIOAction).
 
 Instance mmio_params: MMIO.parameters := { (* everything is inferred automatically *) }.
+
+Existing Instance MinimalMMIOPrimitivesParams. (* needed because it's in a section *)
 
 Instance foo: FlatToRiscv.FlatToRiscv.parameters := _.
 
@@ -93,5 +100,40 @@ Definition zeroedRiscvMachine: RiscvMachine := {|
   getLog := nil;
 |}.
 
+Definition imemStart: word. Admitted. (* TODO *)
+
 Definition initialRiscvMachine(imem: list MachineInt): RiscvMachine :=
-  putProgram imem (word.of_Z 0) zeroedRiscvMachine.
+  putProgram imem imemStart zeroedRiscvMachine.
+
+Definition awesome_postcondition: trace -> Prop. Admitted.
+
+Lemma WP_framework_is_awesome:
+  exec map.empty swap_chars_over_uart nil map.empty map.empty
+       (fun t m l => awesome_postcondition t).
+Admitted.
+
+Definition initialSwapMachine: RiscvMachine :=
+  initialRiscvMachine (List.map encode (compileFunc swap_chars_over_uart)).
+
+(* just to make sure all typeclass instances are available: *)
+Definition mcomp_sat:
+  OStateND RiscvMachine unit -> RiscvMachine -> (RiscvMachine -> Prop) -> Prop :=
+  GoFlatToRiscv.mcomp_sat.
+
+Lemma end2endDemo:
+  runsToNonDet.runsTo (mcomp_sat (run1 RV32IM))
+                      initialSwapMachine
+                      (fun (finalL: RiscvMachine) => awesome_postcondition finalL.(getLog)).
+Proof.
+  (* TODO why does "eapply @exprImp2Riscv_correct" not work? *)
+  unshelve epose proof (@exprImp2Riscv_correct _ _
+    swap_chars_over_uart map.empty _ _ _ imemStart _ _ eq_refl _ _ _ _) as P;
+    [..|eapply P].
+  - cbv - [Z.lt]. (* TODO will need to tighten bounds... *) admit.
+  - cbv. repeat constructor.
+  - reflexivity.
+  - reflexivity.
+  - unfold initialSwapMachine, initialRiscvMachine, getMem.
+    (* TODO relate putProgram to GoFlatToRiscv.program *) admit.
+  - apply WP_framework_is_awesome.
+Admitted.
